experiments on heterogeneous sigma equality

theories/LevelTwo.v
@@ -4,10 +4,10 @@ Module Make (S : Sig).
 Definition arg_ty := @arg_ty (base S.t).
 
 (*********************************************************************************)
-(** *** Terms and substitutions. *)
+(** *** Expressions (terms and substitutions). *)
 (*********************************************************************************)
 
-(** Terms and substitutions are indexed by kinds. *)
+(** Expressions are indexed by kinds. *)
 Inductive kind := 
 | (** Term. *)
   K_t : kind
@@ -19,135 +19,144 @@ Inductive kind :=
   K_s : kind.  
 Derive NoConfusion for kind.
 
-(** Terms and substitutions are indexed by a scope. *)
+(** Expressions are indexed by a scope. *)
 Inductive scope :=
-| (** Scope of a term, argument, or argument list. *)
+| (** Scope of a expr, argument, or argument list. *)
   S1 : nat -> scope
 | (** Scope of a substitution. *)
   S2 : nat -> nat -> scope.
 Derive NoConfusion for scope.
 
-(** A term/substitution metavariable is encoded as a unique identifier (a natural).
-    When denoting a term, we have access to an environment which maps metavariable identifiers
-    to actual (denoted) terms. *)
+(** An expression metavariable is encoded as a unique identifier (a natural).
+    When denoting a expr, we have access to an environment which maps metavariable identifiers
+    to actual (denoted) exprs. *)
 Definition mvar (k : kind) (s : scope) := nat.
 
-(** Terms over an abstract signature. 
-    Terms are indexed by a kind and a scope. *)
-Inductive term : kind -> scope -> Type :=
+#[local] Reserved Notation "'term' n" (at level 0, n at level 0).
+#[local] Reserved Notation "'arg' ty n" (at level 0, ty at level 0, n at level 0).
+#[local] Reserved Notation "'args' tys n" (at level 0, tys at level 0, n at level 0).
+#[local] Reserved Notation "'subst' n m" (at level 50, n at level 0, m at level 0).
+
+(** Expressions over an abstract signature.
+    Expressions are indexed by a kind and a scope. *)
+Inductive expr : kind -> scope -> Type :=
 | (** Term variable. *)
-  T_var {n} : fin n -> term K_t (S1 n)
+  E_var {n} : fin n -> term n
 | (** Non-variable term constructor, applied to a list of arguments. *)
-  T_ctor {n} : forall c, term (K_al (ctor_type S.t c)) (S1 n) -> term K_t (S1 n)
+  E_ctor {n} : forall c, args (ctor_type S.t c) n -> term n
 | (** Empty argument list. *)
-  T_al_nil {n} : term (K_al []) (S1 n)
+  E_al_nil {n} : args [] n
 | (** Non-empty argument list. *)
-  T_al_cons {n ty tys} : term (K_a ty) (S1 n) -> term (K_al tys) (S1 n) -> term (K_al (ty :: tys)) (S1 n)
+  E_al_cons {n ty tys} : arg ty n -> args tys n -> args (ty :: tys) n
 | (** Base argument (e.g. bool or string). *)
-  T_abase {n} : forall b, denote_base S.t b -> term (K_a (AT_base b)) (S1 n)
+  E_abase {n} : forall b, denote_base S.t b -> arg (AT_base b) n
 | (** Term argument. *)
-  T_aterm {n} : term K_t (S1 n) -> term (K_a AT_term) (S1 n)
+  E_aterm {n} : term n -> arg AT_term n
 | (** Binder argument. *)
-  T_abind {n ty} : term (K_a ty) (S1 (S n)) -> term (K_a (AT_bind ty)) (S1 n)
+  E_abind {n ty} : arg ty (S n) -> arg (AT_bind ty) n
 | (** Substitution applied to a term/argument/argument-list. *)
-  T_subst {n m k} : term k (S1 n) -> term K_s (S2 n m) -> term k (S1 m)
+  E_subst {n m k} : expr k (S1 n) -> subst n m -> expr k (S1 m)
 | (** Shift substitution. *)
-  T_sshift {n} : forall k, term K_s (S2 n (k + n))
+  E_sshift {n} : forall k, subst n (k + n)
 | (** Cons substitution. *)
-  T_scons {n m} : term K_t (S1 m) -> term K_s (S2 n m) -> term K_s (S2 (S n) m)
+  E_scons {n m} : term m -> subst n m -> subst (S n) m
 | (** Composition of substitutions. *)
-  T_scomp {n m o} : term K_s (S2 n m) -> term K_s (S2 m o) -> term K_s (S2 n o)
+  E_scomp {n m o} : subst n m -> subst m o -> subst n o
 | (** Metavariable. *)
-  T_mvar {k s} : mvar k s -> term k s.
-Derive Signature NoConfusion for term.
+  E_mvar {k s} : mvar k s -> expr k s
+where "'term' n" := (expr K_t (S1 n))
+  and "'arg' ty n" := (expr (K_a ty) (S1 n))
+  and "'args' tys n" := (expr (K_al tys) (S1 n))
+  and "'subst' n m" := (expr K_s (S2 n m)).
+Derive Signature NoConfusion for expr.
+
+#[local] Notation "↑ k" := (E_sshift k) (at level 0).
+#[local] Notation "t .: s" := (E_scons t s) (at level 60, right associativity).
+#[local] Notation "s1 >> s2" := (E_scomp s1 s2) (at level 50, left associativity).
+#[local] Notation "t '[:' s ']'" := (E_subst t s) (at level 15, s at level 0, no associativity).
 
 (** The identity substitution. *)
-Definition sid {n} : term K_s (S2 n n) := T_sshift 0.
-
-#[local] Notation "↑ k" := (T_sshift k) (at level 0).
-#[local] Notation "t .: s" := (T_scons t s) (at level 60, right associativity).
-#[local] Notation "s1 >> s2" := (T_scomp s1 s2) (at level 50, left associativity).
-#[local] Notation "t '[:' s ']'" := (T_subst t s) (at level 15, s at level 0, no associativity).
+Definition sid {n} : subst n n := E_sshift 0.
 
 (** Lift a substitution through a binder. *)
-Equations up_subst {n m} (s : term K_s (S2 n m)) : term K_s (S2 (S n) (S m)) :=
-up_subst s := T_var fin_zero .: s >> ↑1.
+Equations up_subst {n m} (s : subst n m) : subst (S n) (S m) :=
+up_subst s := E_var fin_zero .: s >> ↑1.
 
 (*********************************************************************************)
 (** *** Axiomatic equality. *)
 (*********************************************************************************)
 
-(** [t =σ t'] means that the terms/substitutions [t] and [t'] are equal 
+(** [e =σ e'] means that the expressions [e] and [e'] are equal 
     modulo the equational theory of sigma calculus. *)
 Reserved Notation "t1 '=σ' t2" (at level 75, no associativity).
-Inductive axiom_eq : forall {k s}, term k s -> term k s -> Prop :=
+Inductive axiom_eq : forall {k s}, expr k s -> expr k s -> Prop :=
 
 (** Equivalence. *)
 
-| aeq_refl {k s} (t : term k s) : t =σ t
-| aeq_sym {k s} (t1 t2 : term k s) : t1 =σ t2 -> t2 =σ t1
-| aeq_trans {k s} (t1 t2 t3 : term k s) : t1 =σ t2 -> t2 =σ t3 -> t1 =σ t3
+| aeq_refl {k s} (e : expr k s) : e =σ e
+| aeq_sym {k s} (e1 e2 : expr k s) : e1 =σ e2 -> e2 =σ e1
+| aeq_trans {k s} (e1 e2 e3 : expr k s) : e1 =σ e2 -> e2 =σ e3 -> e1 =σ e3
 
 (** Congruence. *)
 
-| aeq_congr_ctor {n} c (args1 args2 : term _ (S1 n)) : 
-    args1 =σ args2 -> T_ctor c args1 =σ T_ctor c args2
-| aeq_congr_al_cons {n ty tys} (a1 a2 : term (K_a ty) (S1 n)) (args1 args2 : term (K_al tys) (S1 n)) : 
-    a1 =σ a2 -> args1 =σ args2 -> T_al_cons a1 args1 =σ T_al_cons a2 args2
-| aeq_congr_aterm {n} (t1 t2 : term K_t (S1 n)) : 
-    t1 =σ t2 -> T_aterm t1 =σ T_aterm t2
-| aeq_congr_abind {n ty} (a1 a2 : term (K_a ty) (S1 (S n))) : 
-    a1 =σ a2 -> T_abind a1 =σ T_abind a2
-| aeq_congr_subst {n m k} (t1 t2 : term k (S1 n)) (s1 s2 : term K_s (S2 n m)) : 
+| aeq_congr_ctor {n} c (al1 al2 : args _ n) : 
+    al1 =σ al2 -> E_ctor c al1 =σ E_ctor c al2
+| aeq_congr_al_cons {n ty tys} (a1 a2 : arg ty n) (al1 al2 : args tys n) : 
+    a1 =σ a2 -> al1 =σ al2 -> E_al_cons a1 al1 =σ E_al_cons a2 al2
+| aeq_congr_aterm {n} (t1 t2 : term n) : 
+    t1 =σ t2 -> E_aterm t1 =σ E_aterm t2
+| aeq_congr_abind {n ty} (a1 a2 : arg ty (S n)) : 
+    a1 =σ a2 -> E_abind a1 =σ E_abind a2
+| aeq_congr_subst {n m k} (t1 t2 : expr k (S1 n)) (s1 s2 : subst n m) : 
     t1 =σ t2 -> s1 =σ s2 -> t1[: s1 ] =σ t2[: s2 ] 
-| aeq_congr_scons {n m} (t1 t2 : term K_t (S1 m)) (s1 s2 : term K_s (S2 n m)) : 
+| aeq_congr_scons {n m} (t1 t2 : term m) (s1 s2 : subst n m) : 
     t1 =σ t2 -> s1 =σ s2 -> t1 .: s1 =σ t2 .: s2
-| aeq_congr_scomp {n m o} (s1 s2 : term K_s (S2 n m)) (r1 r2 : term K_s (S2 m o)) : 
+| aeq_congr_scomp {n m o} (s1 s2 : subst n m) (r1 r2 : subst m o) : 
     s1 =σ s2 -> r1 =σ r2 -> s1 >> r1 =σ s2 >> r2
 
 (** Apply a substitution to a variable. *)
 
 | aeq_sshift_var {n} (i : fin n) k : 
-    (T_var i)[: ↑k ] =σ T_var (fin_weaken k i)
-| aeq_scons_zero {n m} (t : term K_t (S1 m)) (s : term K_s (S2 n m)) :
-    (T_var fin_zero)[: t .: s] =σ t
-| aeq_scons_succ {n m} (i : fin n) (t : term K_t (S1 m)) (s : term K_s (S2 n m)) :
-    (T_var (fin_succ i))[: t .: s] =σ (T_var i)[: s]
+    (E_var i)[: ↑k ] =σ E_var (fin_weaken k i)
+| aeq_scons_zero {n m} (t : term m) (s : subst n m) :
+    (E_var fin_zero)[: t .: s] =σ t
+| aeq_scons_succ {n m} (i : fin n) (t : term m) (s : subst n m) :
+    (E_var (fin_succ i))[: t .: s] =σ (E_var i)[: s]
 
-(** Apply a substitution to a term. *)
+(** Apply a substitution to a expr. *)
 
-| aeq_subst_ctor {n m} c (args : term (K_al _) (S1 n)) (s : term K_s (S2 n m)) : 
-    (T_ctor c args)[: s ] =σ T_ctor c (args[: s ])
-| aeq_subst_al_nil {n m} (s : term K_s (S2 n m)) : 
-    T_al_nil[: s ] =σ T_al_nil
-| aeq_subst_al_cons {n m ty tys} (a : term (K_a ty) (S1 n)) (args : term (K_al tys) (S1 n)) (s : term K_s (S2 n m)) : 
-    (T_al_cons a args)[: s ] =σ T_al_cons (a[: s]) (args[: s ])
-| aeq_subst_abase {n m} b x (s : term K_s (S2 n m)) : 
-    (T_abase b x)[: s ] =σ T_abase b x
-| aeq_subst_aterm {n m} (t : term K_t (S1 n)) (s : term K_s (S2 n m)) : 
-    (T_aterm t)[: s ] =σ T_aterm (t[: s ])
-| aeq_subst_abind {n m ty} (a : term (K_a ty) (S1 (S n))) (s : term K_s (S2 n m)) : 
-    (T_abind a)[: s ] =σ T_abind (a[: up_subst s ])
-| aeq_subst_subst {n m o k} (t : term k (S1 n)) (s1 : term K_s (S2 n m)) (s2 : term K_s (S2 m o)) :
+| aeq_subst_ctor {n m} c (al : args _ n) (s : subst n m) : 
+    (E_ctor c al)[: s ] =σ E_ctor c (al[: s ])
+| aeq_subst_al_nil {n m} (s : subst n m) : 
+    E_al_nil[: s ] =σ E_al_nil
+| aeq_subst_al_cons {n m ty tys} (a : arg ty n) (al : args tys n) (s : subst n m) : 
+    (E_al_cons a al)[: s ] =σ E_al_cons (a[: s]) (al[: s ])
+| aeq_subst_abase {n m} b x (s : subst n m) : 
+    (E_abase b x)[: s ] =σ E_abase b x
+| aeq_subst_aterm {n m} (t : term n) (s : subst n m) : 
+    (E_aterm t)[: s ] =σ E_aterm (t[: s ])
+| aeq_subst_abind {n m ty} (a : arg ty (S n)) (s : subst n m) : 
+    (E_abind a)[: s ] =σ E_abind (a[: up_subst s ])
+| aeq_subst_subst {n m o k} (t : expr k (S1 n)) (s1 : subst n m) (s2 : subst m o) :
     t[: s1 ][: s2 ] =σ t[: s1 >> s2 ]
 | aeq_subst_t_mvar {n k} (v : mvar k (S1 n)) :
-    (T_mvar v)[: sid ] =σ T_mvar v 
+    (E_mvar v)[: sid ] =σ E_mvar v 
 
 (** Substitution laws. *)
 
 | aeq_sshift_succ_r {n} k : 
-    ↑k >> ↑1 =σ @T_sshift n (S k)
+    ↑k >> ↑1 =σ @E_sshift n (S k)
 | aeq_sshift_scons {n} :
-    T_var (@fin_zero n) .: ↑1 =σ ↑0  
-| aeq_scons_sshift {n m} (t : term K_t (S1 m)) (s : term K_s (S2 n m)) :
+    E_var (@fin_zero n) .: ↑1 =σ ↑0  
+| aeq_scons_sshift {n m} (t : term m) (s : subst n m) :
   ↑1 >> (t .: s) =σ s
-| aeq_sid_l {n m} (s : term K_s (S2 n m)) : 
+| aeq_sid_l {n m} (s : subst n m) : 
     sid >> s =σ s 
-| aeq_sid_r {n m} (s : term K_s (S2 n m)) : 
+| aeq_sid_r {n m} (s : subst n m) : 
     s >> sid =σ s 
-| aeq_assoc {n m o p} (s1 : term K_s (S2 n m)) (s2 : term K_s (S2 m o)) (s3 : term K_s (S2 o p)) : 
+| aeq_assoc {n m o p} (s1 : subst n m) (s2 : subst m o) (s3 : subst o p) : 
     s1 >> (s2 >> s3) =σ (s1 >> s2) >> s3
-| aeq_distrib {n m o} (t : term K_t (S1 m)) (s1 : term K_s (S2 n m)) (s2 : term K_s (S2 m o)) : 
+| aeq_distrib {n m o} (t : term m) (s1 : subst n m) (s2 : subst m o) : 
     (t .: s1) >> s2 =σ t[: s2 ] .: s1 >> s2
 
 where "t1 '=σ' t2" := (axiom_eq t1 t2).
@@ -160,43 +169,29 @@ Hint Constructors axiom_eq : core.
 #[global] Instance axiom_eq_equiv k s : Equivalence (@axiom_eq k s).
 Proof. constructor ; eauto. Qed.
 
-#[global] Instance t_ctor_proper n c : Proper (axiom_eq ==> axiom_eq) (@T_ctor n c).
+#[global] Instance t_ctor_proper n c : Proper (axiom_eq ==> axiom_eq) (@E_ctor n c).
 Proof. intros ???. apply aeq_congr_ctor ; auto. Qed.
 
-#[global] Instance t_al_cons_proper n ty tys : Proper (axiom_eq ==> axiom_eq ==> axiom_eq) (@T_al_cons n ty tys).
+#[global] Instance t_al_cons_proper n ty tys : Proper (axiom_eq ==> axiom_eq ==> axiom_eq) (@E_al_cons n ty tys).
 Proof. intros ??????. apply aeq_congr_al_cons ; auto. Qed.
 
-#[global] Instance t_aterm_proper n : Proper (axiom_eq ==> axiom_eq) (@T_aterm n).
+#[global] Instance t_aterm_proper n : Proper (axiom_eq ==> axiom_eq) (@E_aterm n).
 Proof. intros ???. apply aeq_congr_aterm ; auto. Qed.
 
-#[global] Instance t_abind_proper n ty : Proper (axiom_eq ==> axiom_eq) (@T_abind n ty).
+#[global] Instance t_abind_proper n ty : Proper (axiom_eq ==> axiom_eq) (@E_abind n ty).
 Proof. intros ???. apply aeq_congr_abind ; auto. Qed.
 
-#[global] Instance t_subst_proper n m k : Proper (axiom_eq ==> axiom_eq ==> axiom_eq) (@T_subst n m k).
+#[global] Instance t_subst_proper n m k : Proper (axiom_eq ==> axiom_eq ==> axiom_eq) (@E_subst n m k).
 Proof. intros ??????. apply aeq_congr_subst ; auto. Qed.
 
-#[global] Instance t_scons_proper n m : Proper (axiom_eq ==> axiom_eq ==> axiom_eq) (@T_scons n m).
+#[global] Instance t_scons_proper n m : Proper (axiom_eq ==> axiom_eq ==> axiom_eq) (@E_scons n m).
 Proof. intros ??????. apply aeq_congr_scons ; auto. Qed.
 
-#[global] Instance t_scomp_proper n m o : Proper (axiom_eq ==> axiom_eq ==> axiom_eq) (@T_scomp n m o).
+#[global] Instance t_scomp_proper n m o : Proper (axiom_eq ==> axiom_eq ==> axiom_eq) (@E_scomp n m o).
 Proof. intros ??????. apply aeq_congr_scomp ; auto. Qed.
 
 (*********************************************************************************)
 (** *** Additional functions and properties. *)
 (*********************************************************************************)
-
-(** Construct an explicit shift by [S k] positions, but with scope [S2 n (k + S n)]
-    instead of [S2 n (S k + n)]. We do this to avoid rewriting with [k + S n = S k + n],
-    which would make proofs harder. *)
-Equations sshift_succ {n} (k : nat) : term K_s (S2 n (k + S n)) :=
-sshift_succ 0 := ↑1 ;
-sshift_succ (S k) := sshift_succ k >> ↑1. 
-
-Lemma aeq_sshift_succ_l {n} k : ↑1 >> ↑k =σ @sshift_succ n k.
-Proof. 
-funelim (sshift_succ k) ; simp sshift_succ.
-- now rewrite aeq_sid_r.
-- rewrite <-H. rewrite <-aeq_assoc. apply t_scomp_proper ; auto.
-Qed. 
 
 End Make.
